books/centaur/vl/loader/find-file.lisp
@@ -20,8 +20,7 @@
 
 (in-package "VL")
 (include-book "../util/warnings")
-(local (include-book "std/io/open-input-channel" :dir :system))
-(local (include-book "std/io/close-input-channel" :dir :system))
+(local (include-book "std/io/base" :dir :system))
 (local (include-book "../util/arithmetic"))
 (set-state-ok t)
 
