books/centaur/vl/loader/read-file.lisp
@@ -21,9 +21,6 @@
 (in-package "VL")
 (include-book "../util/echars")
 (include-book "std/io/base" :dir :system)
-(local (include-book "std/io/open-input-channel" :dir :system))
-(local (include-book "std/io/read-byte" :dir :system))
-(local (include-book "std/io/close-input-channel" :dir :system))
 (local (include-book "../util/arithmetic"))
 (set-state-ok t)
 
