books/std/io/read-ints.lisp
@@ -16,348 +16,19 @@
 ;; Place - Suite 330, Boston, MA 02111-1307, USA.
 
 (in-package "ACL2")
-
-(set-verify-guards-eagerness 2)
-(set-state-ok t)
-
-(include-book "read-byte")
-(local (include-book "unsigned-byte-listp"))
-(local (include-book "signed-byte-listp"))
+(include-book "base")
 (include-book "sign-byte")
 (include-book "combine")
+(local (include-book "unsigned-byte-listp"))
+(local (include-book "signed-byte-listp"))
 (local (include-book "tools/mv-nth" :dir :system))
 (local (include-book "arithmetic-3/bind-free/top" :dir :system))
-
-;; Below are many similar functions, which we have aggregated into the
-;; following macro:
-;;
-;;     (read-bytes$ channel [:bytes bytes]
-;;                          [:signed signed]
-;;                          [:end end])
-;;
-;; If you provide :bytes, it must be either 1, 2, or 4.  (default is 1)
-;; If you provide :signed, it must be either t or nil.   (default is nil)
-;; If you provide :end, it must be either big or little. (default is big)
-;;
-;; The macro simply expands into the appropriate function from the table
-;; below.  (For the 1-byte readers, :end does not matter.)
-;;
-;;     Name         Bytes Read    Value Range        Endian-ness
-;;     read-byte$   1             [0, 2^8-1]         N/A
-;;     read-8s      1             [-2^7, 2^7-1]      N/A
-;;     read-16ube   2             [0, 2^16-1]        Big Endian
-;;     read-16ule   2             [0, 2^16-1]        Little Endian
-;;     read-16sbe   2             [-2^15, 2^15-1]    Big Endian
-;;     read-16sle   2             [-2^15, 2^15-1]    Little Endian
-;;     read-32ube   4             [0, 2^32-1]        Big Endian
-;;     read-32ule   4             [0, 2^32-1]        Little Endian
-;;     read-32sbe   4             [-2^32, 2^32-1]    Big Endian
-;;     read-32sle   4             [-2^32, 2^32-1]    Little Endian
-;;
-;; We also provide another macro which allows you to read a fixed sequence of
-;; same-length quantifies.  The interface is very similar to the above:
-;;
-;;     (read-bytes$-n n channel [:bytes bytes]
-;;                              [:signed signed]
-;;                              [:end end])
-;;
-;; Here n must be a natural number, while :bytes, :signed, and :end must
-;; conform to the same restrictions as before.  The macro expands to a list
-;; version of the appropriate function, which is logically a simple recursion
-;; until n reaches zero, but under the hood is implemented in a tail recursive
-;; manner for greater efficiency.
-;;
-;; These functions return fail if EOF is reached before (n * bytes) are read
-;; from the stream.  Otherwise, they return an n-element list where every
-;; member is constructed in accordance with the table above.
-
-
+(set-verify-guards-eagerness 2)
+(set-state-ok t)
 
 (local (defthm rationalp-when-integerp
          (implies (integerp x)
                   (rationalp x))))
-
-
-;; read-8s
-
-(defun read-8s (channel state)
-  "Read a signed byte from an input channel."
-  (declare (xargs :guard (and (state-p state)
-                              (symbolp channel)
-                              (open-input-channel-p channel :byte state))
-                  :verify-guards nil))
-  (mv-let (byte state)
-          (read-byte$ channel state)
-          (if byte
-              (mv (mbe :logic (sign-byte byte)
-                       :exec  (if (< (the-fixnum byte) 128)
-                                  byte
-                                (the-fixnum
-                                 (- (the-fixnum byte) 256))))
-                  state)
-            (mv nil state))))
-
-(verify-guards read-8s
-  :hints(("Goal" :in-theory (enable sign-byte signed-byte-p))))
-
-(defthm read-8s-signed-byte
-  (implies (and (mv-nth 0 (read-8s channel state))
-                (force (state-p1 state))
-                (force (open-input-channel-p1 channel :byte state))
-                (force (symbolp channel)))
-           (signed-byte-p 8 (mv-nth 0 (read-8s channel state)))))
-
-(defthm read-8s-integer
-  (implies (and (mv-nth 0 (read-8s channel state))
-                (force (state-p1 state))
-                (force (open-input-channel-p1 channel :byte state))
-                (force (symbolp channel)))
-           (integerp (mv-nth 0 (read-8s channel state)))))
-
-(defthm read-8s-range
-  (implies (and (mv-nth 0 (read-8s channel state))
-                (force (state-p1 state))
-                (force (open-input-channel-p1 channel :byte state))
-                (force (symbolp channel)))
-           (and (<= -128 (mv-nth 0 (read-8s channel state)))
-                (<= (- (expt 2 7)) (mv-nth 0 (read-8s channel state)))
-                (< (mv-nth 0 (read-8s channel state)) 128)
-                (< (mv-nth 0 (read-8s channel state)) (expt 2 7))))
-  :rule-classes :linear
-  :hints(("Goal"
-          :in-theory (enable signed-byte-p)
-          :use (:instance read-8s-signed-byte))))
-
-(defthm read-8s-state
-  (implies (and (force (state-p1 state))
-                (force (open-input-channel-p1 channel :byte state))
-                (force (symbolp channel)))
-           (state-p1 (mv-nth 1 (read-8s channel state)))))
-
-(defthm read-8s-open-input-channel-p1
-  (implies (and (force (state-p1 state))
-                (force (open-input-channel-p1 channel :byte state))
-                (force (symbolp channel)))
-           (open-input-channel-p1 channel
-                                  :byte
-                                  (mv-nth 1 (read-8s channel state)))))
-
-(in-theory (disable read-8s))
-
-
-;; read-16ube
-
-(defun read-16ube (channel state)
-  (declare (xargs :guard (and (state-p state)
-                              (symbolp channel)
-                              (open-input-channel-p channel :byte state))
-                  :guard-hints(("Goal" :in-theory (enable combine16u)))))
-  (mv-let (x1 state) (read-byte$ channel state)
-  (mv-let (x2 state) (read-byte$ channel state)
-  (if (null x1)
-      (mv nil state)
-    (if (null x2)
-        (mv 'fail state)
-      (mv (mbe :logic (combine16u x1 x2)
-               :exec (logior
-                      (the (unsigned-byte 16)
-                        (ash (the (unsigned-byte 8) x1) 8))
-                      (the (unsigned-byte 8)
-                        x2)))
-          state))))))
-
-(defthm read-16ube-unsigned-byte
-  (implies (and (force (state-p1 state))
-                (force (open-input-channel-p1 channel :byte state))
-                (force (symbolp channel))
-                (mv-nth 0 (read-16ube channel state))
-                (not (equal (mv-nth 0 (read-16ube channel state)) 'fail)))
-           (unsigned-byte-p 16 (mv-nth 0 (read-16ube channel state)))))
-
-(defthm read-16ube-integer
-  (implies (and (force (state-p1 state))
-                (force (open-input-channel-p1 channel :byte state))
-                (force (symbolp channel))
-                (mv-nth 0 (read-16ube channel state))
-                (not (equal (mv-nth 0 (read-16ube channel state)) 'fail)))
-           (integerp (mv-nth 0 (read-16ube channel state)))))
-
-(defthm read-16ube-range
-  (implies (and (force (state-p1 state))
-                (force (open-input-channel-p1 channel :byte state))
-                (force (symbolp channel))
-                (mv-nth 0 (read-16ube channel state))
-                (not (equal (mv-nth 0 (read-16ube channel state)) 'fail)))
-           (and (<= 0 (mv-nth 0 (read-16ube channel state)))
-                (< (mv-nth 0 (read-16ube channel state)) 65536)
-                (< (mv-nth 0 (read-16ube channel state)) (expt 2 16))))
-  :rule-classes :linear
-  :hints(("Goal"
-          :in-theory (enable unsigned-byte-p)
-          :use (:instance read-16ube-unsigned-byte))))
-
-(defthm read-16ube-state
-  (implies (and (force (state-p1 state))
-                (force (open-input-channel-p1 channel :byte state))
-                (force (symbolp channel)))
-           (state-p1 (mv-nth 1 (read-16ube channel state)))))
-
-(defthm read-16ube-open-input-channel-p1
-  (implies (and (force (state-p1 state))
-                (force (open-input-channel-p1 channel :byte state))
-                (force (symbolp channel)))
-           (open-input-channel-p1 channel
-                                  :byte
-                                  (mv-nth 1 (read-16ube channel state)))))
-
-(in-theory (disable read-16ube))
-
-
-
-;; read-16ule
-
-(defun read-16ule (channel state)
-  (declare (xargs :guard (and (state-p state)
-                              (symbolp channel)
-                              (open-input-channel-p channel :byte state))
-                  :guard-hints(("Goal" :in-theory (enable combine16u)))))
-  (mv-let (x1 state) (read-byte$ channel state)
-  (mv-let (x2 state) (read-byte$ channel state)
-  (if (null x1)
-      (mv nil state)
-    (if (null x2)
-        (mv 'fail state)
-      (mv (mbe :logic (combine16u x2 x1)
-               :exec (logior
-                      (the (unsigned-byte 16)
-                        (ash (the (unsigned-byte 8) x2) 8))
-                      (the (unsigned-byte 8)
-                        x1)))
-          state))))))
-
-(defthm read-16ule-unsigned-byte
-  (implies (and (force (state-p1 state))
-                (force (open-input-channel-p1 channel :byte state))
-                (force (symbolp channel))
-                (mv-nth 0 (read-16ule channel state))
-                (not (equal (mv-nth 0 (read-16ule channel state)) 'fail)))
-           (unsigned-byte-p 16 (mv-nth 0 (read-16ule channel state)))))
-
-(defthm read-16ule-integer
-  (implies (and (force (state-p1 state))
-                (force (open-input-channel-p1 channel :byte state))
-                (force (symbolp channel))
-                (mv-nth 0 (read-16ule channel state))
-                (not (equal (mv-nth 0 (read-16ule channel state)) 'fail)))
-           (integerp (mv-nth 0 (read-16ule channel state)))))
-
-(defthm read-16ule-range
-  (implies (and (force (state-p1 state))
-                (force (open-input-channel-p1 channel :byte state))
-                (force (symbolp channel))
-                (mv-nth 0 (read-16ule channel state))
-                (not (equal (mv-nth 0 (read-16ule channel state)) 'fail)))
-           (and (<= 0 (mv-nth 0 (read-16ule channel state)))
-                (< (mv-nth 0 (read-16ule channel state)) 65536)
-                (< (mv-nth 0 (read-16ule channel state)) (expt 2 16))))
-  :rule-classes :linear
-  :hints(("Goal"
-          :in-theory (enable unsigned-byte-p)
-          :use (:instance read-16ule-unsigned-byte))))
-
-(defthm read-16ule-state
-  (implies (and (force (state-p1 state))
-                (force (open-input-channel-p1 channel :byte state))
-                (force (symbolp channel)))
-           (state-p1 (mv-nth 1 (read-16ule channel state)))))
-
-(defthm read-16ule-open-input-channel-p1
-  (implies (and (force (state-p1 state))
-                (force (open-input-channel-p1 channel :byte state))
-                (force (symbolp channel)))
-           (open-input-channel-p1 channel
-                                  :byte
-                                  (mv-nth 1 (read-16ule channel state)))))
-
-(in-theory (disable read-16ule))
-
-
-
-;; read-16sbe
-
-(defun read-16sbe (channel state)
-  (declare (xargs :guard (and (state-p state)
-                              (symbolp channel)
-                              (open-input-channel-p channel :byte state))
-                  :guard-hints(("Goal" :in-theory (enable combine16s sign-byte)))))
-  (mv-let (x1 state) (read-byte$ channel state)
-  (mv-let (x2 state) (read-byte$ channel state)
-  (if (null x1)
-      (mv nil state)
-    (if (null x2)
-        (mv 'fail state)
-      (mv (mbe :logic (combine16s x1 x2)
-               :exec (logior (the (signed-byte 16)
-                                  (ash (the (signed-byte 8)
-                                            (if (< (the-fixnum x1) 128)
-                                                (the-fixnum x1)
-                                              (the-fixnum
-                                               (- (the-fixnum x1) 256))))
-                                       8))
-                             (the (unsigned-byte 8)
-                                  x2)))
-          state))))))
-
-(defthm read-16sbe-signed-byte
-  (implies (and (force (state-p1 state))
-                (force (open-input-channel-p1 channel :byte state))
-                (force (symbolp channel))
-                (mv-nth 0 (read-16sbe channel state))
-                (not (equal (mv-nth 0 (read-16sbe channel state)) 'fail)))
-           (signed-byte-p 16 (mv-nth 0 (read-16sbe channel state)))))
-
-(defthm read-16sbe-integer
-  (implies (and (force (state-p1 state))
-                (force (open-input-channel-p1 channel :byte state))
-                (force (symbolp channel))
-                (mv-nth 0 (read-16sbe channel state))
-                (not (equal (mv-nth 0 (read-16sbe channel state)) 'fail)))
-           (integerp (mv-nth 0 (read-16sbe channel state)))))
-
-(defthm read-16sbe-range
-  (implies (and (force (state-p1 state))
-                (force (open-input-channel-p1 channel :byte state))
-                (force (symbolp channel))
-                (mv-nth 0 (read-16sbe channel state))
-                (not (equal (mv-nth 0 (read-16sbe channel state)) 'fail)))
-           (and (<= -32768 (mv-nth 0 (read-16sbe channel state)))
-                (<= (- (expt 2 15)) (mv-nth 0 (read-16sbe channel state)))
-                (< (mv-nth 0 (read-16sbe channel state)) 32768)
-                (< (mv-nth 0 (read-16sbe channel state)) (expt 2 15))))
-  :rule-classes :linear
-  :hints(("Goal"
-          :in-theory (enable signed-byte-p)
-          :use (:instance read-16sbe-signed-byte))))
-
-(defthm read-16sbe-state
-  (implies (and (force (state-p1 state))
-                (force (open-input-channel-p1 channel :byte state))
-                (force (symbolp channel)))
-           (state-p1 (mv-nth 1 (read-16sbe channel state)))))
-
-(defthm read-16sbe-open-input-channel-p1
-  (implies (and (force (state-p1 state))
-                (force (open-input-channel-p1 channel :byte state))
-                (force (symbolp channel)))
-           (open-input-channel-p1 channel
-                                  :byte
-                                  (mv-nth 1 (read-16sbe channel state)))))
-
-(in-theory (disable read-16sbe))
-
-
-
-;; read-16sle
 
 #+non-standard-analysis
 (local
@@ -365,448 +36,957 @@
    (implies (integerp x)
 	    (realp x))))
 
-(defun read-16sle (channel state)
-  (declare (xargs :guard (and (state-p state)
-                              (symbolp channel)
-                              (open-input-channel-p channel :byte state))
-                  :guard-hints(("Goal" :in-theory (enable combine16s sign-byte)))))
-  (mv-let (x1 state) (read-byte$ channel state)
-  (mv-let (x2 state) (read-byte$ channel state)
-  (if (null x1)
-      (mv nil state)
-    (if (null x2)
-        (mv 'fail state)
-      (mv (mbe :logic (combine16s x2 x1)
-               :exec (logior (the (signed-byte 16)
-                                  (ash (the (signed-byte 8)
-                                            (if (< (the-fixnum x2) 128)
-                                                (the-fixnum x2)
-                                              (the-fixnum
-                                               (- (the-fixnum x2) 256))))
-                                       8))
-                             (the (unsigned-byte 8)
-                                  x1)))
-          state))))))
+(local (defthm unsigned-byte-p-of-read-byte$
+         (implies (and (state-p1 state)
+                       (open-input-channel-p1 channel :byte state))
+                  (b* (((mv x1 ?state) (read-byte$ channel state)))
+                    (iff (unsigned-byte-p 8 x1)
+                         x1)))))
 
-(defthm read-16sle-signed-byte
-  (implies (and (force (state-p1 state))
-                (force (open-input-channel-p1 channel :byte state))
-                (force (symbolp channel))
-                (mv-nth 0 (read-16sle channel state))
-                (not (equal (mv-nth 0 (read-16sle channel state)) 'fail)))
-           (signed-byte-p 16 (mv-nth 0 (read-16sle channel state)))))
+(local (defthm read-byte$-returns-plenty-of-nils-after-eof
+         (implies (and (state-p1 state)
+                       (open-input-channel-p1 channel :byte state))
+                  (b* (((mv x1 state) (read-byte$ channel state))
+                       ((mv x2 ?state) (read-byte$ channel state)))
+                    (implies x2 x1)))))
 
-(defthm read-16sle-integer
-  (implies (and (force (state-p1 state))
-                (force (open-input-channel-p1 channel :byte state))
-                (force (symbolp channel))
-                (mv-nth 0 (read-16sle channel state))
-                (not (equal (mv-nth 0 (read-16sle channel state)) 'fail)))
-           (integerp (mv-nth 0 (read-16sle channel state)))))
-
-(defthm read-16sle-range
-  (implies (and (force (state-p1 state))
-                (force (open-input-channel-p1 channel :byte state))
-                (force (symbolp channel))
-                (mv-nth 0 (read-16sle channel state))
-                (not (equal (mv-nth 0 (read-16sle channel state)) 'fail)))
-           (and (<= -32768 (mv-nth 0 (read-16sle channel state)))
-                (<= (- (expt 2 15)) (mv-nth 0 (read-16sle channel state)))
-                (< (mv-nth 0 (read-16sle channel state)) 32768)
-                (< (mv-nth 0 (read-16sle channel state)) (expt 2 15))))
-  :rule-classes :linear
-  :hints(("Goal"
-          :in-theory (enable signed-byte-p)
-          :use (:instance read-16sle-signed-byte))))
-
-(defthm read-16sle-state
-  (implies (and (force (state-p1 state))
-                (force (open-input-channel-p1 channel :byte state))
-                (force (symbolp channel)))
-           (state-p1 (mv-nth 1 (read-16sle channel state)))))
-
-(defthm read-16sle-open-input-channel-p1
-  (implies (and (force (state-p1 state))
-                (force (open-input-channel-p1 channel :byte state))
-                (force (symbolp channel)))
-           (open-input-channel-p1 channel
-                                  :byte
-                                  (mv-nth 1 (read-16sle channel state)))))
-
-(in-theory (disable read-16sle))
+;; There's no read-8u since that's just read-byte$.
 
 
+(defsection read-8s
+  :parents (read-bytes$)
+  :short "@(call read-8s) reads a signed byte from the input channel."
 
-;; read-32ube
+  (defund read-8s (channel state)
+    (declare (xargs :guard (and (state-p state)
+                                (symbolp channel)
+                                (open-input-channel-p channel :byte state))))
+    (b* (((mv byte state) (read-byte$ channel state))
+         ((unless byte)
+          (mv nil state)))
+      (mv (sign-byte byte) state)))
 
-(defun read-32ube (channel state)
-  (declare (xargs :guard (and (state-p state)
-                              (symbolp channel)
-                              (open-input-channel-p channel :byte state))
-                  :guard-hints(("Goal" :in-theory (enable combine32u)))))
-  (mv-let (x1 state) (read-byte$ channel state)
-  (mv-let (x2 state) (read-byte$ channel state)
-  (mv-let (x3 state) (read-byte$ channel state)
-  (mv-let (x4 state) (read-byte$ channel state)
-  (if (null x1)
-      (mv nil state)
-    (if (or (null x2) (null x3) (null x4))
-        (mv 'fail state)
-      (mv (mbe :logic (combine32u x1 x2 x3 x4)
-               :exec (logior (the (unsigned-byte 32)
-                               (ash (the (unsigned-byte 8) x1) 24))
-                      (the (unsigned-byte 24)
-                           (logior
-                             (the (unsigned-byte 24)
-                               (ash (the (unsigned-byte 8) x2) 16))
-                             (the (unsigned-byte 16)
-                                  (logior
-                                   (the (unsigned-byte 16)
-                                        (ash (the (unsigned-byte 8) x3) 8))
-                                   (the (unsigned-byte 8)
-                                        x4)))))))
-          state))))))))
+  (local (in-theory (enable read-8s)))
 
-(defthm read-32ube-unsigned-byte
-  (implies (and (force (state-p1 state))
-                (force (open-input-channel-p1 channel :byte state))
-                (force (symbolp channel))
-                (mv-nth 0 (read-32ube channel state))
-                (not (equal (mv-nth 0 (read-32ube channel state)) 'fail)))
-           (unsigned-byte-p 32 (mv-nth 0 (read-32ube channel state)))))
+  (defthm read-8s-signed-byte
+    (implies (and (mv-nth 0 (read-8s channel state))
+                  (force (state-p1 state))
+                  (force (open-input-channel-p1 channel :byte state))
+                  (force (symbolp channel)))
+             (signed-byte-p 8 (mv-nth 0 (read-8s channel state)))))
 
-(defthm read-32ube-integer
-  (implies (and (force (state-p1 state))
-                (force (open-input-channel-p1 channel :byte state))
-                (force (symbolp channel))
-                (mv-nth 0 (read-32ube channel state))
-                (not (equal (mv-nth 0 (read-32ube channel state)) 'fail)))
-           (integerp (mv-nth 0 (read-32ube channel state)))))
+  (defthm read-8s-integer
+    (implies (mv-nth 0 (read-8s channel state))
+             (integerp (mv-nth 0 (read-8s channel state)))))
 
-(defthm read-32ube-range
-  (implies (and (force (state-p1 state))
-                (force (open-input-channel-p1 channel :byte state))
-                (force (symbolp channel))
-                (mv-nth 0 (read-32ube channel state))
-                (not (equal (mv-nth 0 (read-32ube channel state)) 'fail)))
-           (and (<= 0 (mv-nth 0 (read-32ube channel state)))
-                (< (mv-nth 0 (read-32ube channel state)) 4294967296)
-                (< (mv-nth 0 (read-32ube channel state)) (expt 2 32))))
-  :rule-classes :linear
-  :hints(("Goal"
-          :in-theory (enable unsigned-byte-p)
-          :use (:instance read-32ube-unsigned-byte))))
+  (defthm read-8s-range
+    (implies (and (mv-nth 0 (read-8s channel state))
+                  (force (state-p1 state))
+                  (force (open-input-channel-p1 channel :byte state))
+                  (force (symbolp channel)))
+             (and (<= -128 (mv-nth 0 (read-8s channel state)))
+                  (<= (- (expt 2 7)) (mv-nth 0 (read-8s channel state)))
+                  (< (mv-nth 0 (read-8s channel state)) 128)
+                  (< (mv-nth 0 (read-8s channel state)) (expt 2 7))))
+    :rule-classes :linear
+    :hints(("Goal"
+            :in-theory (enable signed-byte-p)
+            :use (:instance read-8s-signed-byte))))
 
-(defthm read-32ube-state
-  (implies (and (force (state-p1 state))
-                (force (open-input-channel-p1 channel :byte state))
-                (force (symbolp channel)))
-           (state-p1 (mv-nth 1 (read-32ube channel state)))))
+  (defthm read-8s-state
+    (implies (and (force (state-p1 state))
+                  (force (open-input-channel-p1 channel :byte state))
+                  (force (symbolp channel)))
+             (state-p1 (mv-nth 1 (read-8s channel state)))))
 
-(defthm read-32ube-open-input-channel-p1
-  (implies (and (force (state-p1 state))
-                (force (open-input-channel-p1 channel :byte state))
-                (force (symbolp channel)))
-           (open-input-channel-p1 channel
-                                  :byte
-                                  (mv-nth 1 (read-32ube channel state)))))
-
-(in-theory (disable read-32ube))
+  (defthm read-8s-open-input-channel-p1
+    (implies (and (force (state-p1 state))
+                  (force (open-input-channel-p1 channel :byte state))
+                  (force (symbolp channel)))
+             (open-input-channel-p1 channel
+                                    :byte
+                                    (mv-nth 1 (read-8s channel state))))))
 
 
+(defsection read-16ube
+  :parents (read-bytes$)
+  :short "@(call read-16ube) reads a 16-bit, unsigned, big-endian value from
+the input channel."
 
-;; read-32ule
+  (defund read-16ube (channel state)
+    (declare (xargs :guard (and (state-p state)
+                                (symbolp channel)
+                                (open-input-channel-p channel :byte state))))
+    (b* (((mv x1 state) (read-byte$ channel state))
+         ((mv x2 state) (read-byte$ channel state))
+         ((unless x1)
+          (mv nil state))
+         ((unless x2)
+          (mv 'fail state)))
+      (mv (combine16u x1 x2) state)))
 
-(defun read-32ule (channel state)
-  (declare (xargs :guard (and (state-p state)
-                              (symbolp channel)
-                              (open-input-channel-p channel :byte state))
-                  :guard-hints(("Goal" :in-theory (enable combine32u)))))
-  (mv-let (x1 state) (read-byte$ channel state)
-  (mv-let (x2 state) (read-byte$ channel state)
-  (mv-let (x3 state) (read-byte$ channel state)
-  (mv-let (x4 state) (read-byte$ channel state)
-  (if (null x1)
-      (mv nil state)
-    (if (or (null x2) (null x3) (null x4))
-        (mv 'fail state)
-      (mv (mbe :logic (combine32u x4 x3 x2 x1)
-               :exec (logior (the (unsigned-byte 32)
-                               (ash (the (unsigned-byte 8) x4) 24))
-                             (the (unsigned-byte 24)
-                                  (logior
-                                   (the (unsigned-byte 24)
-                                        (ash (the (unsigned-byte 8) x3) 16))
-                                   (the (unsigned-byte 16)
-                                        (logior
-                                         (the (unsigned-byte 16)
-                                              (ash (the (unsigned-byte 8) x2) 8))
-                                         (the (unsigned-byte 8)
-                                              x1)))))))
-          state))))))))
+  (local (in-theory (enable read-16ube)))
 
-(defthm read-32ule-unsigned-byte
-  (implies (and (force (state-p1 state))
-                (force (open-input-channel-p1 channel :byte state))
-                (force (symbolp channel))
-                (mv-nth 0 (read-32ule channel state))
-                (not (equal (mv-nth 0 (read-32ule channel state)) 'fail)))
-           (unsigned-byte-p 32 (mv-nth 0 (read-32ule channel state)))))
+  (defthm read-16ube-unsigned-byte
+    (implies (and (force (state-p1 state))
+                  (force (open-input-channel-p1 channel :byte state))
+                  (force (symbolp channel))
+                  (mv-nth 0 (read-16ube channel state))
+                  (not (equal (mv-nth 0 (read-16ube channel state)) 'fail)))
+             (unsigned-byte-p 16 (mv-nth 0 (read-16ube channel state)))))
 
-(defthm read-32ule-integer
-  (implies (and (force (state-p1 state))
-                (force (open-input-channel-p1 channel :byte state))
-                (force (symbolp channel))
-                (mv-nth 0 (read-32ule channel state))
-                (not (equal (mv-nth 0 (read-32ule channel state)) 'fail)))
-           (integerp (mv-nth 0 (read-32ule channel state)))))
+  (defthm read-16ube-integer
+    (implies (and (mv-nth 0 (read-16ube channel state))
+                  (not (equal (mv-nth 0 (read-16ube channel state)) 'fail)))
+             (integerp (mv-nth 0 (read-16ube channel state)))))
 
-(defthm read-32ule-range
-  (implies (and (force (state-p1 state))
-                (force (open-input-channel-p1 channel :byte state))
-                (force (symbolp channel))
-                (mv-nth 0 (read-32ule channel state))
-                (not (equal (mv-nth 0 (read-32ule channel state)) 'fail)))
-           (and (<= 0 (mv-nth 0 (read-32ule channel state)))
-                (< (mv-nth 0 (read-32ule channel state)) 4294967296)
-                (< (mv-nth 0 (read-32ule channel state)) (expt 2 32))))
-  :rule-classes :linear
-  :hints(("Goal"
-          :in-theory (enable unsigned-byte-p)
-          :use (:instance read-32ule-unsigned-byte))))
+  (defthm read-16ube-range
+    (implies (and (force (state-p1 state))
+                  (force (open-input-channel-p1 channel :byte state))
+                  (force (symbolp channel))
+                  (mv-nth 0 (read-16ube channel state))
+                  (not (equal (mv-nth 0 (read-16ube channel state)) 'fail)))
+             (and (<= 0 (mv-nth 0 (read-16ube channel state)))
+                  (< (mv-nth 0 (read-16ube channel state)) 65536)
+                  (< (mv-nth 0 (read-16ube channel state)) (expt 2 16))))
+    :rule-classes :linear
+    :hints(("Goal"
+            :in-theory (enable unsigned-byte-p)
+            :use (:instance read-16ube-unsigned-byte))))
 
-(defthm read-32ule-state
-  (implies (and (force (state-p1 state))
-                (force (open-input-channel-p1 channel :byte state))
-                (force (symbolp channel)))
-           (state-p1 (mv-nth 1 (read-32ule channel state)))))
+  (defthm read-16ube-state
+    (implies (and (force (state-p1 state))
+                  (force (open-input-channel-p1 channel :byte state))
+                  (force (symbolp channel)))
+             (state-p1 (mv-nth 1 (read-16ube channel state)))))
 
-(defthm read-32ule-open-input-channel-p1
-  (implies (and (force (state-p1 state))
-                (force (open-input-channel-p1 channel :byte state))
-                (force (symbolp channel)))
-           (open-input-channel-p1 channel
-                                  :byte
-                                  (mv-nth 1 (read-32ule channel state)))))
-
-(in-theory (disable read-32ule))
+  (defthm read-16ube-open-input-channel-p1
+    (implies (and (force (state-p1 state))
+                  (force (open-input-channel-p1 channel :byte state))
+                  (force (symbolp channel)))
+             (open-input-channel-p1 channel
+                                    :byte
+                                    (mv-nth 1 (read-16ube channel state))))))
 
 
+(defsection read-16ule
+  :parents (read-bytes$)
+  :short "@(call read-16ule) reads a 16-bit, unsigned, little-endian value
+from the input channel."
 
-;; read-32sbe
+  (defund read-16ule (channel state)
+    (declare (xargs :guard (and (state-p state)
+                                (symbolp channel)
+                                (open-input-channel-p channel :byte state))))
+    (b* (((mv x1 state) (read-byte$ channel state))
+         ((mv x2 state) (read-byte$ channel state))
+         ((unless x1)
+          (mv nil state))
+         ((unless x2)
+          (mv 'fail state)))
+      (mv (combine16u x2 x1) state)))
 
-(defun read-32sbe (channel state)
-  (declare (xargs :guard (and (state-p state)
-                              (symbolp channel)
-                              (open-input-channel-p channel :byte state))
-                  :guard-hints(("Goal" :in-theory (enable combine32s sign-byte)))))
-  (mv-let (x1 state) (read-byte$ channel state)
-  (mv-let (x2 state) (read-byte$ channel state)
-  (mv-let (x3 state) (read-byte$ channel state)
-  (mv-let (x4 state) (read-byte$ channel state)
-  (if (null x1)
-      (mv nil state)
-    (if (or (null x2) (null x3) (null x4))
-        (mv 'fail state)
-      (mv (mbe :logic (combine32s x1 x2 x3 x4)
-               :exec (logior (the (signed-byte 32)
-                               (ash (the (signed-byte 8)
-                                         (if (< (the-fixnum x1) 128)
-                                             x1
-                                           (the-fixnum
-                                            (- (the-fixnum x1) 256))))
-                                    24))
-                             (the (unsigned-byte 24)
-                                  (logior
-                                   (the (unsigned-byte 24)
-                                        (ash (the (unsigned-byte 8) x2) 16))
-                                   (the (unsigned-byte 16)
-                                        (logior
-                                         (the (unsigned-byte 16)
-                                              (ash (the (unsigned-byte 8) x3) 8))
-                                         (the (unsigned-byte 8)
-                                              x4)))))))
-          state))))))))
+  (local (in-theory (enable read-16ule)))
 
-(defthm read-32sbe-signed-byte
-  (implies (and (force (state-p1 state))
-                (force (open-input-channel-p1 channel :byte state))
-                (force (symbolp channel))
-                (mv-nth 0 (read-32sbe channel state))
-                (not (equal (mv-nth 0 (read-32sbe channel state)) 'fail)))
-           (signed-byte-p 32 (mv-nth 0 (read-32sbe channel state)))))
+  (defthm read-16ule-unsigned-byte
+    (implies (and (force (state-p1 state))
+                  (force (open-input-channel-p1 channel :byte state))
+                  (force (symbolp channel))
+                  (mv-nth 0 (read-16ule channel state))
+                  (not (equal (mv-nth 0 (read-16ule channel state)) 'fail)))
+             (unsigned-byte-p 16 (mv-nth 0 (read-16ule channel state)))))
 
-(defthm read-32sbe-integer
-  (implies (and (force (state-p1 state))
-                (force (open-input-channel-p1 channel :byte state))
-                (force (symbolp channel))
-                (mv-nth 0 (read-32sbe channel state))
-                (not (equal (mv-nth 0 (read-32sbe channel state)) 'fail)))
-           (integerp (mv-nth 0 (read-32sbe channel state)))))
+  (defthm read-16ule-integer
+    (implies (and (mv-nth 0 (read-16ule channel state))
+                  (not (equal (mv-nth 0 (read-16ule channel state)) 'fail)))
+             (integerp (mv-nth 0 (read-16ule channel state)))))
 
-(defthm read-32sbe-range
-  (implies (and (force (state-p1 state))
-                (force (open-input-channel-p1 channel :byte state))
-                (force (symbolp channel))
-                (mv-nth 0 (read-32sbe channel state))
-                (not (equal (mv-nth 0 (read-32sbe channel state)) 'fail)))
-           (and (<= -2147483648 (mv-nth 0 (read-32sbe channel state)))
-                (<= (- (expt 2 31)) (mv-nth 0 (read-32sbe channel state)))
-                (< (mv-nth 0 (read-32sbe channel state)) 2147483648)
-                (< (mv-nth 0 (read-32sbe channel state)) (expt 2 31))))
-  :rule-classes :linear
-  :hints(("Goal"
-          :in-theory (enable signed-byte-p)
-          :use (:instance read-32sbe-signed-byte))))
+  (defthm read-16ule-range
+    (implies (and (force (state-p1 state))
+                  (force (open-input-channel-p1 channel :byte state))
+                  (force (symbolp channel))
+                  (mv-nth 0 (read-16ule channel state))
+                  (not (equal (mv-nth 0 (read-16ule channel state)) 'fail)))
+             (and (<= 0 (mv-nth 0 (read-16ule channel state)))
+                  (< (mv-nth 0 (read-16ule channel state)) 65536)
+                  (< (mv-nth 0 (read-16ule channel state)) (expt 2 16))))
+    :rule-classes :linear
+    :hints(("Goal"
+            :in-theory (enable unsigned-byte-p)
+            :use (:instance read-16ule-unsigned-byte))))
 
-(defthm read-32sbe-state
-  (implies (and (force (state-p1 state))
-                (force (open-input-channel-p1 channel :byte state))
-                (force (symbolp channel)))
-           (state-p1 (mv-nth 1 (read-32sbe channel state)))))
+  (defthm read-16ule-state
+    (implies (and (force (state-p1 state))
+                  (force (open-input-channel-p1 channel :byte state))
+                  (force (symbolp channel)))
+             (state-p1 (mv-nth 1 (read-16ule channel state)))))
 
-(defthm read-32sbe-open-input-channel-p1
-  (implies (and (force (state-p1 state))
-                (force (open-input-channel-p1 channel :byte state))
-                (force (symbolp channel)))
-           (open-input-channel-p1 channel
-                                  :byte
-                                  (mv-nth 1 (read-32sbe channel state)))))
-
-(in-theory (disable read-32sbe))
+  (defthm read-16ule-open-input-channel-p1
+    (implies (and (force (state-p1 state))
+                  (force (open-input-channel-p1 channel :byte state))
+                  (force (symbolp channel)))
+             (open-input-channel-p1 channel
+                                    :byte
+                                    (mv-nth 1 (read-16ule channel state))))))
 
 
+(defsection read-16sbe
+  :parents (read-bytes$)
+  :short "@(call read-16sbe) reads a 16-bit, signed, big-endian value from the
+input channel."
 
-;; read-32sle
+  (defund read-16sbe (channel state)
+    (declare (xargs :guard (and (state-p state)
+                                (symbolp channel)
+                                (open-input-channel-p channel :byte state))))
+    (b* (((mv x1 state) (read-byte$ channel state))
+         ((mv x2 state) (read-byte$ channel state))
+         ((unless x1)
+          (mv nil state))
+         ((unless x2)
+          (mv 'fail state)))
+      (mv (combine16s x1 x2) state)))
 
-(defun read-32sle (channel state)
-  (declare (xargs :guard (and (state-p state)
-                              (symbolp channel)
-                              (open-input-channel-p channel :byte state))
-                  :guard-hints(("Goal" :in-theory (enable combine32s sign-byte)))))
-  (mv-let (x1 state) (read-byte$ channel state)
-  (mv-let (x2 state) (read-byte$ channel state)
-  (mv-let (x3 state) (read-byte$ channel state)
-  (mv-let (x4 state) (read-byte$ channel state)
-  (if (null x1)
-      (mv nil state)
-    (if (or (null x2) (null x3) (null x4))
-        (mv 'fail state)
-      (mv (mbe :logic (combine32s x4 x3 x2 x1)
-               :exec (logior (the (signed-byte 32)
-                               (ash (the (signed-byte 8)
-                                         (if (< (the-fixnum x4) 128)
-                                             x4
-                                           (the-fixnum
-                                            (- (the-fixnum x4) 256))))
-                                    24))
-                             (the (unsigned-byte 24)
-                                  (logior
-                                   (the (unsigned-byte 24)
-                                        (ash (the (unsigned-byte 8) x3) 16))
-                                   (the (unsigned-byte 16)
-                                        (logior
-                                         (the (unsigned-byte 16)
-                                              (ash (the (unsigned-byte 8) x2) 8))
-                                         (the (unsigned-byte 8)
-                                              x1)))))))
-          state))))))))
+  (local (in-theory (enable read-16sbe)))
 
-(defthm read-32sle-signed-byte
-  (implies (and (force (state-p1 state))
-                (force (open-input-channel-p1 channel :byte state))
-                (force (symbolp channel))
-                (mv-nth 0 (read-32sle channel state))
-                (not (equal (mv-nth 0 (read-32sle channel state)) 'fail)))
-           (signed-byte-p 32 (mv-nth 0 (read-32sle channel state)))))
+  (defthm read-16sbe-signed-byte
+    (implies (and (force (state-p1 state))
+                  (force (open-input-channel-p1 channel :byte state))
+                  (force (symbolp channel))
+                  (mv-nth 0 (read-16sbe channel state))
+                  (not (equal (mv-nth 0 (read-16sbe channel state)) 'fail)))
+             (signed-byte-p 16 (mv-nth 0 (read-16sbe channel state)))))
 
-(defthm read-32sle-integer
-  (implies (and (force (state-p1 state))
-                (force (open-input-channel-p1 channel :byte state))
-                (force (symbolp channel))
-                (mv-nth 0 (read-32sle channel state))
-                (not (equal (mv-nth 0 (read-32sle channel state)) 'fail)))
-           (integerp (mv-nth 0 (read-32sle channel state)))))
+  (defthm read-16sbe-integer
+    (implies (and (mv-nth 0 (read-16sbe channel state))
+                  (not (equal (mv-nth 0 (read-16sbe channel state)) 'fail)))
+             (integerp (mv-nth 0 (read-16sbe channel state)))))
 
-(defthm read-32sle-range
-  (implies (and (force (state-p1 state))
-                (force (open-input-channel-p1 channel :byte state))
-                (force (symbolp channel))
-                (mv-nth 0 (read-32sle channel state))
-                (not (equal (mv-nth 0 (read-32sle channel state)) 'fail)))
-           (and (<= -2147483648 (mv-nth 0 (read-32sle channel state)))
-                (<= (- (expt 2 31)) (mv-nth 0 (read-32sle channel state)))
-                (< (mv-nth 0 (read-32sle channel state)) 2147483648)
-                (< (mv-nth 0 (read-32sle channel state)) (expt 2 31))))
-  :rule-classes :linear
-  :hints(("Goal"
-          :in-theory (enable signed-byte-p)
-          :use (:instance read-32sle-signed-byte))))
+  (defthm read-16sbe-range
+    (implies (and (force (state-p1 state))
+                  (force (open-input-channel-p1 channel :byte state))
+                  (force (symbolp channel))
+                  (mv-nth 0 (read-16sbe channel state))
+                  (not (equal (mv-nth 0 (read-16sbe channel state)) 'fail)))
+             (and (<= -32768 (mv-nth 0 (read-16sbe channel state)))
+                  (<= (- (expt 2 15)) (mv-nth 0 (read-16sbe channel state)))
+                  (< (mv-nth 0 (read-16sbe channel state)) 32768)
+                  (< (mv-nth 0 (read-16sbe channel state)) (expt 2 15))))
+    :rule-classes :linear
+    :hints(("Goal"
+            :in-theory (enable signed-byte-p)
+            :use (:instance read-16sbe-signed-byte))))
 
-(defthm read-32sle-state
-  (implies (and (force (state-p1 state))
-                (force (open-input-channel-p1 channel :byte state))
-                (force (symbolp channel)))
-           (state-p1 (mv-nth 1 (read-32sle channel state)))))
+  (defthm read-16sbe-state
+    (implies (and (force (state-p1 state))
+                  (force (open-input-channel-p1 channel :byte state))
+                  (force (symbolp channel)))
+             (state-p1 (mv-nth 1 (read-16sbe channel state)))))
 
-(defthm read-32sle-open-input-channel-p1
-  (implies (and (force (state-p1 state))
-                (force (open-input-channel-p1 channel :byte state))
-                (force (symbolp channel)))
-           (open-input-channel-p1 channel
-                                  :byte
-                                  (mv-nth 1 (read-32sle channel state)))))
+  (defthm read-16sbe-open-input-channel-p1
+    (implies (and (force (state-p1 state))
+                  (force (open-input-channel-p1 channel :byte state))
+                  (force (symbolp channel)))
+             (open-input-channel-p1 channel
+                                    :byte
+                                    (mv-nth 1 (read-16sbe channel state))))))
 
-(in-theory (disable read-32sle))
+
+(defsection read-16sle
+  :parents (read-bytes$)
+  :short "@(call read-16sle) reads a 16-bit, signed, little-endian value from
+the input channel."
+
+  (defund read-16sle (channel state)
+    (declare (xargs :guard (and (state-p state)
+                                (symbolp channel)
+                                (open-input-channel-p channel :byte state))))
+    (b* (((mv x1 state) (read-byte$ channel state))
+         ((mv x2 state) (read-byte$ channel state))
+         ((unless x1)
+          (mv nil state))
+         ((unless x2)
+          (mv 'fail state)))
+      (mv (combine16s x2 x1) state)))
+
+  (local (in-theory (enable read-16sle)))
+
+  (defthm read-16sle-signed-byte
+    (implies (and (force (state-p1 state))
+                  (force (open-input-channel-p1 channel :byte state))
+                  (force (symbolp channel))
+                  (mv-nth 0 (read-16sle channel state))
+                  (not (equal (mv-nth 0 (read-16sle channel state)) 'fail)))
+             (signed-byte-p 16 (mv-nth 0 (read-16sle channel state)))))
+
+  (defthm read-16sle-integer
+    (implies (and (mv-nth 0 (read-16sle channel state))
+                  (not (equal (mv-nth 0 (read-16sle channel state)) 'fail)))
+             (integerp (mv-nth 0 (read-16sle channel state)))))
+
+  (defthm read-16sle-range
+    (implies (and (force (state-p1 state))
+                  (force (open-input-channel-p1 channel :byte state))
+                  (force (symbolp channel))
+                  (mv-nth 0 (read-16sle channel state))
+                  (not (equal (mv-nth 0 (read-16sle channel state)) 'fail)))
+             (and (<= -32768 (mv-nth 0 (read-16sle channel state)))
+                  (<= (- (expt 2 15)) (mv-nth 0 (read-16sle channel state)))
+                  (< (mv-nth 0 (read-16sle channel state)) 32768)
+                  (< (mv-nth 0 (read-16sle channel state)) (expt 2 15))))
+    :rule-classes :linear
+    :hints(("Goal"
+            :in-theory (enable signed-byte-p)
+            :use (:instance read-16sle-signed-byte))))
+
+  (defthm read-16sle-state
+    (implies (and (force (state-p1 state))
+                  (force (open-input-channel-p1 channel :byte state))
+                  (force (symbolp channel)))
+             (state-p1 (mv-nth 1 (read-16sle channel state)))))
+
+  (defthm read-16sle-open-input-channel-p1
+    (implies (and (force (state-p1 state))
+                  (force (open-input-channel-p1 channel :byte state))
+                  (force (symbolp channel)))
+             (open-input-channel-p1 channel
+                                    :byte
+                                    (mv-nth 1 (read-16sle channel state))))))
 
 
 
-;; read-bytes$ macro
+(defsection read-32ube
+  :parents (read-bytes$)
+  :short "@(call read-32ube) reads a 32-bit, unsigned, big-endian value from
+the input channel."
 
-(defmacro read-bytes$ (channel &key (bytes '1)
-                                    (signed 'nil)
-                                    (end 'big))
-  (declare (xargs :guard (and (symbolp channel)
-                              (booleanp signed)
-                              (or (equal bytes 1)
-                                  (equal bytes 2)
-                                  (equal bytes 4))
-                              (or (equal end 'little)
-                                  (equal end 'big)))))
-  (case end
-    ('big (if signed
+  (defund read-32ube (channel state)
+    (declare (xargs :guard (and (state-p state)
+                                (symbolp channel)
+                                (open-input-channel-p channel :byte state))))
+    (b* (((mv x1 state) (read-byte$ channel state))
+         ((mv x2 state) (read-byte$ channel state))
+         ((mv x3 state) (read-byte$ channel state))
+         ((mv x4 state) (read-byte$ channel state))
+         ((unless x1)
+          (mv nil state))
+         ((unless x4)
+          (mv 'fail state)))
+      (mv (combine32u x1 x2 x3 x4) state)))
+
+  (local (in-theory (enable read-32ube)))
+
+  (defthm read-32ube-unsigned-byte
+    (implies (and (force (state-p1 state))
+                  (force (open-input-channel-p1 channel :byte state))
+                  (force (symbolp channel))
+                  (mv-nth 0 (read-32ube channel state))
+                  (not (equal (mv-nth 0 (read-32ube channel state)) 'fail)))
+             (unsigned-byte-p 32 (mv-nth 0 (read-32ube channel state)))))
+
+  (defthm read-32ube-integer
+    (implies (and (mv-nth 0 (read-32ube channel state))
+                  (not (equal (mv-nth 0 (read-32ube channel state)) 'fail)))
+             (integerp (mv-nth 0 (read-32ube channel state)))))
+
+  (defthm read-32ube-range
+    (implies (and (force (state-p1 state))
+                  (force (open-input-channel-p1 channel :byte state))
+                  (force (symbolp channel))
+                  (mv-nth 0 (read-32ube channel state))
+                  (not (equal (mv-nth 0 (read-32ube channel state)) 'fail)))
+             (and (<= 0 (mv-nth 0 (read-32ube channel state)))
+                  (< (mv-nth 0 (read-32ube channel state)) 4294967296)
+                  (< (mv-nth 0 (read-32ube channel state)) (expt 2 32))))
+    :rule-classes :linear
+    :hints(("Goal"
+            :in-theory (enable unsigned-byte-p)
+            :use (:instance read-32ube-unsigned-byte))))
+
+  (defthm read-32ube-state
+    (implies (and (force (state-p1 state))
+                  (force (open-input-channel-p1 channel :byte state))
+                  (force (symbolp channel)))
+             (state-p1 (mv-nth 1 (read-32ube channel state)))))
+
+  (defthm read-32ube-open-input-channel-p1
+    (implies (and (force (state-p1 state))
+                  (force (open-input-channel-p1 channel :byte state))
+                  (force (symbolp channel)))
+             (open-input-channel-p1 channel
+                                    :byte
+                                    (mv-nth 1 (read-32ube channel state))))))
+
+
+
+(defsection read-32ule
+  :parents (read-bytes$)
+  :short "@(call read-32ule) reads a 32-bit, unsigned, little-endian value
+from the input channel."
+
+  (defund read-32ule (channel state)
+    (declare (xargs :guard (and (state-p state)
+                                (symbolp channel)
+                                (open-input-channel-p channel :byte state))))
+    (b* (((mv x1 state) (read-byte$ channel state))
+         ((mv x2 state) (read-byte$ channel state))
+         ((mv x3 state) (read-byte$ channel state))
+         ((mv x4 state) (read-byte$ channel state))
+         ((unless x1)
+          (mv nil state))
+         ((unless x4)
+          (mv 'fail state)))
+      (mv (combine32u x4 x3 x2 x1) state)))
+
+  (local (in-theory (enable read-32ule)))
+
+  (defthm read-32ule-unsigned-byte
+    (implies (and (force (state-p1 state))
+                  (force (open-input-channel-p1 channel :byte state))
+                  (force (symbolp channel))
+                  (mv-nth 0 (read-32ule channel state))
+                  (not (equal (mv-nth 0 (read-32ule channel state)) 'fail)))
+             (unsigned-byte-p 32 (mv-nth 0 (read-32ule channel state)))))
+
+  (defthm read-32ule-integer
+    (implies (and (force (state-p1 state))
+                  (force (open-input-channel-p1 channel :byte state))
+                  (force (symbolp channel))
+                  (mv-nth 0 (read-32ule channel state))
+                  (not (equal (mv-nth 0 (read-32ule channel state)) 'fail)))
+             (integerp (mv-nth 0 (read-32ule channel state)))))
+
+  (defthm read-32ule-range
+    (implies (and (force (state-p1 state))
+                  (force (open-input-channel-p1 channel :byte state))
+                  (force (symbolp channel))
+                  (mv-nth 0 (read-32ule channel state))
+                  (not (equal (mv-nth 0 (read-32ule channel state)) 'fail)))
+             (and (<= 0 (mv-nth 0 (read-32ule channel state)))
+                  (< (mv-nth 0 (read-32ule channel state)) 4294967296)
+                  (< (mv-nth 0 (read-32ule channel state)) (expt 2 32))))
+    :rule-classes :linear
+    :hints(("Goal"
+            :in-theory (enable unsigned-byte-p)
+            :use (:instance read-32ule-unsigned-byte))))
+
+  (defthm read-32ule-state
+    (implies (and (force (state-p1 state))
+                  (force (open-input-channel-p1 channel :byte state))
+                  (force (symbolp channel)))
+             (state-p1 (mv-nth 1 (read-32ule channel state)))))
+
+  (defthm read-32ule-open-input-channel-p1
+    (implies (and (force (state-p1 state))
+                  (force (open-input-channel-p1 channel :byte state))
+                  (force (symbolp channel)))
+             (open-input-channel-p1 channel
+                                    :byte
+                                    (mv-nth 1 (read-32ule channel state))))))
+
+
+(defsection read-32sbe
+  :parents (read-bytes$)
+  :short "@(call read-32sbe) reads a 32-bit, signed, big-endian value from the
+input channel."
+
+  (defund read-32sbe (channel state)
+    (declare (xargs :guard (and (state-p state)
+                                (symbolp channel)
+                                (open-input-channel-p channel :byte state))))
+    (b* (((mv x1 state) (read-byte$ channel state))
+         ((mv x2 state) (read-byte$ channel state))
+         ((mv x3 state) (read-byte$ channel state))
+         ((mv x4 state) (read-byte$ channel state))
+         ((unless x1)
+          (mv nil state))
+         ((unless x4)
+          (mv 'fail state)))
+      (mv (combine32s x1 x2 x3 x4) state)))
+
+  (local (in-theory (enable read-32sbe)))
+
+  (defthm read-32sbe-signed-byte
+    (implies (and (force (state-p1 state))
+                  (force (open-input-channel-p1 channel :byte state))
+                  (force (symbolp channel))
+                  (mv-nth 0 (read-32sbe channel state))
+                  (not (equal (mv-nth 0 (read-32sbe channel state)) 'fail)))
+             (signed-byte-p 32 (mv-nth 0 (read-32sbe channel state)))))
+
+  (defthm read-32sbe-integer
+    (implies (and (mv-nth 0 (read-32sbe channel state))
+                  (not (equal (mv-nth 0 (read-32sbe channel state)) 'fail)))
+             (integerp (mv-nth 0 (read-32sbe channel state)))))
+
+  (defthm read-32sbe-range
+    (implies (and (force (state-p1 state))
+                  (force (open-input-channel-p1 channel :byte state))
+                  (force (symbolp channel))
+                  (mv-nth 0 (read-32sbe channel state))
+                  (not (equal (mv-nth 0 (read-32sbe channel state)) 'fail)))
+             (and (<= -2147483648 (mv-nth 0 (read-32sbe channel state)))
+                  (<= (- (expt 2 31)) (mv-nth 0 (read-32sbe channel state)))
+                  (< (mv-nth 0 (read-32sbe channel state)) 2147483648)
+                  (< (mv-nth 0 (read-32sbe channel state)) (expt 2 31))))
+    :rule-classes :linear
+    :hints(("Goal"
+            :in-theory (enable signed-byte-p)
+            :use (:instance read-32sbe-signed-byte))))
+
+  (defthm read-32sbe-state
+    (implies (and (force (state-p1 state))
+                  (force (open-input-channel-p1 channel :byte state))
+                  (force (symbolp channel)))
+             (state-p1 (mv-nth 1 (read-32sbe channel state)))))
+
+  (defthm read-32sbe-open-input-channel-p1
+    (implies (and (force (state-p1 state))
+                  (force (open-input-channel-p1 channel :byte state))
+                  (force (symbolp channel)))
+             (open-input-channel-p1 channel
+                                    :byte
+                                    (mv-nth 1 (read-32sbe channel state))))))
+
+
+(defsection read-32sle
+  :parents (read-bytes$)
+  :short "@(call read-32sle) reads a 32-bit, signed, little-endian value from
+the input channel."
+
+  (defund read-32sle (channel state)
+    (declare (xargs :guard (and (state-p state)
+                                (symbolp channel)
+                                (open-input-channel-p channel :byte state))))
+    (b* (((mv x1 state) (read-byte$ channel state))
+         ((mv x2 state) (read-byte$ channel state))
+         ((mv x3 state) (read-byte$ channel state))
+         ((mv x4 state) (read-byte$ channel state))
+         ((unless x1)
+          (mv nil state))
+         ((unless x4)
+          (mv 'fail state)))
+      (mv (combine32s x4 x3 x2 x1) state)))
+
+  (local (in-theory (enable read-32sle)))
+
+  (defthm read-32sle-signed-byte
+    (implies (and (force (state-p1 state))
+                  (force (open-input-channel-p1 channel :byte state))
+                  (force (symbolp channel))
+                  (mv-nth 0 (read-32sle channel state))
+                  (not (equal (mv-nth 0 (read-32sle channel state)) 'fail)))
+             (signed-byte-p 32 (mv-nth 0 (read-32sle channel state)))))
+
+  (defthm read-32sle-integer
+    (implies (and (mv-nth 0 (read-32sle channel state))
+                  (not (equal (mv-nth 0 (read-32sle channel state)) 'fail)))
+             (integerp (mv-nth 0 (read-32sle channel state)))))
+
+  (defthm read-32sle-range
+    (implies (and (force (state-p1 state))
+                  (force (open-input-channel-p1 channel :byte state))
+                  (force (symbolp channel))
+                  (mv-nth 0 (read-32sle channel state))
+                  (not (equal (mv-nth 0 (read-32sle channel state)) 'fail)))
+             (and (<= -2147483648 (mv-nth 0 (read-32sle channel state)))
+                  (<= (- (expt 2 31)) (mv-nth 0 (read-32sle channel state)))
+                  (< (mv-nth 0 (read-32sle channel state)) 2147483648)
+                  (< (mv-nth 0 (read-32sle channel state)) (expt 2 31))))
+    :rule-classes :linear
+    :hints(("Goal"
+            :in-theory (enable signed-byte-p)
+            :use (:instance read-32sle-signed-byte))))
+
+  (defthm read-32sle-state
+    (implies (and (force (state-p1 state))
+                  (force (open-input-channel-p1 channel :byte state))
+                  (force (symbolp channel)))
+             (state-p1 (mv-nth 1 (read-32sle channel state)))))
+
+  (defthm read-32sle-open-input-channel-p1
+    (implies (and (force (state-p1 state))
+                  (force (open-input-channel-p1 channel :byte state))
+                  (force (symbolp channel)))
+             (open-input-channel-p1 channel
+                                    :byte
+                                    (mv-nth 1 (read-32sle channel state))))))
+
+
+
+(defsection read-64ube
+  :parents (read-bytes$)
+  :short "@(call read-64ube) reads a 64-bit, unsigned, big-endian value from
+the input channel."
+
+  (defund read-64ube (channel state)
+    (declare (xargs :guard (and (state-p state)
+                                (symbolp channel)
+                                (open-input-channel-p channel :byte state))))
+    (b* (((mv x1 state) (read-byte$ channel state))
+         ((mv x2 state) (read-byte$ channel state))
+         ((mv x3 state) (read-byte$ channel state))
+         ((mv x4 state) (read-byte$ channel state))
+         ((mv x5 state) (read-byte$ channel state))
+         ((mv x6 state) (read-byte$ channel state))
+         ((mv x7 state) (read-byte$ channel state))
+         ((mv x8 state) (read-byte$ channel state))
+         ((unless x1)
+          (mv nil state))
+         ((unless x8)
+          (mv 'fail state)))
+      (mv (combine64u x1 x2 x3 x4 x5 x6 x7 x8) state)))
+
+  (local (in-theory (enable read-64ube)))
+
+  (defthm read-64ube-unsigned-byte
+    (implies (and (force (state-p1 state))
+                  (force (open-input-channel-p1 channel :byte state))
+                  (force (symbolp channel))
+                  (mv-nth 0 (read-64ube channel state))
+                  (not (equal (mv-nth 0 (read-64ube channel state)) 'fail)))
+             (unsigned-byte-p 64 (mv-nth 0 (read-64ube channel state)))))
+
+  (defthm read-64ube-integer
+    (implies (and (mv-nth 0 (read-64ube channel state))
+                  (not (equal (mv-nth 0 (read-64ube channel state)) 'fail)))
+             (integerp (mv-nth 0 (read-64ube channel state)))))
+
+  (defthm read-64ube-range
+    (implies (and (force (state-p1 state))
+                  (force (open-input-channel-p1 channel :byte state))
+                  (force (symbolp channel))
+                  (mv-nth 0 (read-64ube channel state))
+                  (not (equal (mv-nth 0 (read-64ube channel state)) 'fail)))
+             (and (<= 0 (mv-nth 0 (read-64ube channel state)))
+                  (< (mv-nth 0 (read-64ube channel state)) 18446744073709551616)
+                  (< (mv-nth 0 (read-64ube channel state)) (expt 2 64))))
+    :rule-classes :linear
+    :hints(("Goal"
+            :in-theory (enable unsigned-byte-p)
+            :use (:instance read-64ube-unsigned-byte))))
+
+  (defthm read-64ube-state
+    (implies (and (force (state-p1 state))
+                  (force (open-input-channel-p1 channel :byte state))
+                  (force (symbolp channel)))
+             (state-p1 (mv-nth 1 (read-64ube channel state)))))
+
+  (defthm read-64ube-open-input-channel-p1
+    (implies (and (force (state-p1 state))
+                  (force (open-input-channel-p1 channel :byte state))
+                  (force (symbolp channel)))
+             (open-input-channel-p1 channel
+                                    :byte
+                                    (mv-nth 1 (read-64ube channel state))))))
+
+
+
+(defsection read-64ule
+  :parents (read-bytes$)
+  :short "@(call read-64ule) reads a 64-bit, unsigned, little-endian value from
+the input channel."
+
+  (defund read-64ule (channel state)
+    (declare (xargs :guard (and (state-p state)
+                                (symbolp channel)
+                                (open-input-channel-p channel :byte state))))
+    (b* (((mv x1 state) (read-byte$ channel state))
+         ((mv x2 state) (read-byte$ channel state))
+         ((mv x3 state) (read-byte$ channel state))
+         ((mv x4 state) (read-byte$ channel state))
+         ((mv x5 state) (read-byte$ channel state))
+         ((mv x6 state) (read-byte$ channel state))
+         ((mv x7 state) (read-byte$ channel state))
+         ((mv x8 state) (read-byte$ channel state))
+         ((unless x1)
+          (mv nil state))
+         ((unless x8)
+          (mv 'fail state)))
+      (mv (combine64u x8 x7 x6 x5 x4 x3 x2 x1) state)))
+
+  (local (in-theory (enable read-64ule)))
+
+  (defthm read-64ule-unsigned-byte
+    (implies (and (force (state-p1 state))
+                  (force (open-input-channel-p1 channel :byte state))
+                  (force (symbolp channel))
+                  (mv-nth 0 (read-64ule channel state))
+                  (not (equal (mv-nth 0 (read-64ule channel state)) 'fail)))
+             (unsigned-byte-p 64 (mv-nth 0 (read-64ule channel state)))))
+
+  (defthm read-64ule-integer
+    (implies (and (mv-nth 0 (read-64ule channel state))
+                  (not (equal (mv-nth 0 (read-64ule channel state)) 'fail)))
+             (integerp (mv-nth 0 (read-64ule channel state)))))
+
+  (defthm read-64ule-range
+    (implies (and (force (state-p1 state))
+                  (force (open-input-channel-p1 channel :byte state))
+                  (force (symbolp channel))
+                  (mv-nth 0 (read-64ule channel state))
+                  (not (equal (mv-nth 0 (read-64ule channel state)) 'fail)))
+             (and (<= 0 (mv-nth 0 (read-64ule channel state)))
+                  (< (mv-nth 0 (read-64ule channel state)) 18446744073709551616)
+                  (< (mv-nth 0 (read-64ule channel state)) (expt 2 64))))
+    :rule-classes :linear
+    :hints(("Goal"
+            :in-theory (enable unsigned-byte-p)
+            :use (:instance read-64ule-unsigned-byte))))
+
+  (defthm read-64ule-state
+    (implies (and (force (state-p1 state))
+                  (force (open-input-channel-p1 channel :byte state))
+                  (force (symbolp channel)))
+             (state-p1 (mv-nth 1 (read-64ule channel state)))))
+
+  (defthm read-64ule-open-input-channel-p1
+    (implies (and (force (state-p1 state))
+                  (force (open-input-channel-p1 channel :byte state))
+                  (force (symbolp channel)))
+             (open-input-channel-p1 channel
+                                    :byte
+                                    (mv-nth 1 (read-64ule channel state))))))
+
+
+(defsection read-64sbe
+  :parents (read-bytes$)
+  :short "@(call read-64sbe) reads a 64-bit, signed, big-endian value from the
+input channel."
+
+  (defund read-64sbe (channel state)
+    (declare (xargs :guard (and (state-p state)
+                                (symbolp channel)
+                                (open-input-channel-p channel :byte state))))
+    (b* (((mv x1 state) (read-byte$ channel state))
+         ((mv x2 state) (read-byte$ channel state))
+         ((mv x3 state) (read-byte$ channel state))
+         ((mv x4 state) (read-byte$ channel state))
+         ((mv x5 state) (read-byte$ channel state))
+         ((mv x6 state) (read-byte$ channel state))
+         ((mv x7 state) (read-byte$ channel state))
+         ((mv x8 state) (read-byte$ channel state))
+         ((unless x1)
+          (mv nil state))
+         ((unless x8)
+          (mv 'fail state)))
+      (mv (combine64s x1 x2 x3 x4 x5 x6 x7 x8) state)))
+
+  (local (in-theory (enable read-64sbe)))
+
+  (defthm read-64sbe-signed-byte
+    (implies (and (force (state-p1 state))
+                  (force (open-input-channel-p1 channel :byte state))
+                  (force (symbolp channel))
+                  (mv-nth 0 (read-64sbe channel state))
+                  (not (equal (mv-nth 0 (read-64sbe channel state)) 'fail)))
+             (signed-byte-p 64 (mv-nth 0 (read-64sbe channel state)))))
+
+  (defthm read-64sbe-integer
+    (implies (and (mv-nth 0 (read-64sbe channel state))
+                  (not (equal (mv-nth 0 (read-64sbe channel state)) 'fail)))
+             (integerp (mv-nth 0 (read-64sbe channel state)))))
+
+  (defthm read-64sbe-range
+    (implies (and (force (state-p1 state))
+                  (force (open-input-channel-p1 channel :byte state))
+                  (force (symbolp channel))
+                  (mv-nth 0 (read-64sbe channel state))
+                  (not (equal (mv-nth 0 (read-64sbe channel state)) 'fail)))
+             (and (<= -9223372036854775808 (mv-nth 0 (read-64sbe channel state)))
+                  (<= (- (expt 2 63)) (mv-nth 0 (read-64sbe channel state)))
+                  (< (mv-nth 0 (read-64sbe channel state)) 9223372036854775808)
+                  (< (mv-nth 0 (read-64sbe channel state)) (expt 2 63))))
+    :rule-classes :linear
+    :hints(("Goal"
+            :in-theory (enable signed-byte-p)
+            :use (:instance read-64sbe-signed-byte))))
+
+  (defthm read-64sbe-state
+    (implies (and (force (state-p1 state))
+                  (force (open-input-channel-p1 channel :byte state))
+                  (force (symbolp channel)))
+             (state-p1 (mv-nth 1 (read-64sbe channel state)))))
+
+  (defthm read-64sbe-open-input-channel-p1
+    (implies (and (force (state-p1 state))
+                  (force (open-input-channel-p1 channel :byte state))
+                  (force (symbolp channel)))
+             (open-input-channel-p1 channel
+                                    :byte
+                                    (mv-nth 1 (read-64sbe channel state))))))
+
+
+(defsection read-64sle
+  :parents (read-bytes$)
+  :short "@(call read-64sle) reads a 64-bit, signed, big-endian value from the
+input channel."
+
+  (defund read-64sle (channel state)
+    (declare (xargs :guard (and (state-p state)
+                                (symbolp channel)
+                                (open-input-channel-p channel :byte state))))
+    (b* (((mv x1 state) (read-byte$ channel state))
+         ((mv x2 state) (read-byte$ channel state))
+         ((mv x3 state) (read-byte$ channel state))
+         ((mv x4 state) (read-byte$ channel state))
+         ((mv x5 state) (read-byte$ channel state))
+         ((mv x6 state) (read-byte$ channel state))
+         ((mv x7 state) (read-byte$ channel state))
+         ((mv x8 state) (read-byte$ channel state))
+         ((unless x1)
+          (mv nil state))
+         ((unless x8)
+          (mv 'fail state)))
+      (mv (combine64s x8 x7 x6 x5 x4 x3 x2 x1) state)))
+
+  (local (in-theory (enable read-64sle)))
+
+  (defthm read-64sle-signed-byte
+    (implies (and (force (state-p1 state))
+                  (force (open-input-channel-p1 channel :byte state))
+                  (force (symbolp channel))
+                  (mv-nth 0 (read-64sle channel state))
+                  (not (equal (mv-nth 0 (read-64sle channel state)) 'fail)))
+             (signed-byte-p 64 (mv-nth 0 (read-64sle channel state)))))
+
+  (defthm read-64sle-integer
+    (implies (and (mv-nth 0 (read-64sle channel state))
+                  (not (equal (mv-nth 0 (read-64sle channel state)) 'fail)))
+             (integerp (mv-nth 0 (read-64sle channel state)))))
+
+  (defthm read-64sle-range
+    (implies (and (force (state-p1 state))
+                  (force (open-input-channel-p1 channel :byte state))
+                  (force (symbolp channel))
+                  (mv-nth 0 (read-64sle channel state))
+                  (not (equal (mv-nth 0 (read-64sle channel state)) 'fail)))
+             (and (<= -9223372036854775808 (mv-nth 0 (read-64sle channel state)))
+                  (<= (- (expt 2 63)) (mv-nth 0 (read-64sle channel state)))
+                  (< (mv-nth 0 (read-64sle channel state)) 9223372036854775808)
+                  (< (mv-nth 0 (read-64sle channel state)) (expt 2 63))))
+    :rule-classes :linear
+    :hints(("Goal"
+            :in-theory (enable signed-byte-p)
+            :use (:instance read-64sle-signed-byte))))
+
+  (defthm read-64sle-state
+    (implies (and (force (state-p1 state))
+                  (force (open-input-channel-p1 channel :byte state))
+                  (force (symbolp channel)))
+             (state-p1 (mv-nth 1 (read-64sle channel state)))))
+
+  (defthm read-64sle-open-input-channel-p1
+    (implies (and (force (state-p1 state))
+                  (force (open-input-channel-p1 channel :byte state))
+                  (force (symbolp channel)))
+             (open-input-channel-p1 channel
+                                    :byte
+                                    (mv-nth 1 (read-64sle channel state))))))
+
+
+(defsection read-bytes$
+  :parents (io)
+  :short "Flexible macro for reading and combining 1, 2, 4, or 8 bytes from an
+open @(':byte') input stream into a single value."
+
+  :long "<p>General form:</p>
+@({
+     (read-bytes$ channel
+                  [:bytes bytes]    ;; default: 1
+                  [:signed signed]  ;; default: nil
+                  [:end end]        ;; default: big
+                  )
+       -->
+     (mv value state)
+})
+
+<ul>
+
+<li>If you provide @('bytes'), it must be explicitly 1, 2, 4, or 8.</li>
+
+<li>If you provide @('signed'), it must be either t or nil.</li>
+
+<li>If you provide @('end'), it must be either big or little. (For the 1-byte
+readers, :end does not matter.)</li>
+
+</ul>
+
+<p>This is a macro that expands into the appropriate function from the table
+below.</p>
+
+@({
+     Name         Bytes Read    Value Range        Endian-ness
+   ---------------------------------------------------------------
+     read-byte$   1             [0, 2^8-1]         N/A
+     read-8s      1             [-2^7, 2^7-1]      N/A
+
+     read-16ube   2             [0, 2^16-1]        Big Endian
+     read-16ule   2             [0, 2^16-1]        Little Endian
+     read-16sbe   2             [-2^15, 2^15-1]    Big Endian
+     read-16sle   2             [-2^15, 2^15-1]    Little Endian
+
+     read-32ube   4             [0, 2^32-1]        Big Endian
+     read-32ule   4             [0, 2^32-1]        Little Endian
+     read-32sbe   4             [-2^31, 2^31-1]    Big Endian
+     read-32sle   4             [-2^31, 2^31-1]    Little Endian
+
+     read-64ube   8             [0, 2^64-1]        Big Endian
+     read-64ule   8             [0, 2^64-1]        Little Endian
+     read-64sbe   8             [-2^63, 2^63-1]    Big Endian
+     read-64sle   8             [-2^63, 2^63-1]    Little Endian
+   ---------------------------------------------------------------
+})"
+
+  (defmacro read-bytes$ (channel &key
+                                 (bytes '1)
+                                 (signed 'nil)
+                                 (end 'big))
+    (declare (xargs :guard (and (symbolp channel)
+                                (booleanp signed)
+                                (or (equal bytes 1)
+                                    (equal bytes 2)
+                                    (equal bytes 4))
+                                (or (equal end 'little)
+                                    (equal end 'big)))))
+    (case end
+      ('big (if signed
+                (case bytes
+                  (1 `(read-8s ,channel state))
+                  (2 `(read-16sbe ,channel state))
+                  (4 `(read-32sbe ,channel state))
+                  (8 `(read-64sbe ,channel state))
+                  (t (er hard 'read-bytes$ "Bad case in read-bytes$.")))
               (case bytes
-                (1 `(read-8s ,channel state))
-                (2 `(read-16sbe ,channel state))
-                (4 `(read-32sbe ,channel state))
-                (t (er hard 'read-bytes$ "Bad case in read-bytes$.")))
-            (case bytes
-              (1 `(read-byte$ ,channel state))
-              (2 `(read-16ube ,channel state))
-              (4 `(read-32ube ,channel state))
-              (t (er hard 'read-bytes$ "Bad case in read-bytes$.")))))
-    ('little (if signed
+                (1 `(read-byte$ ,channel state))
+                (2 `(read-16ube ,channel state))
+                (4 `(read-32ube ,channel state))
+                (8 `(read-64ube ,channel state))
+                (t (er hard 'read-bytes$ "Bad case in read-bytes$.")))))
+      ('little (if signed
+                   (case bytes
+                     (1 `(read-8s ,channel state))
+                     (2 `(read-16sle ,channel state))
+                     (4 `(read-32sle ,channel state))
+                     (8 `(read-64sle ,channel state))
+                     (t (er hard 'read-bytes$ "Bad case in read-bytes$.")))
                  (case bytes
-                   (1 `(read-8s ,channel state))
-                   (2 `(read-16sle ,channel state))
-                   (4 `(read-32sle ,channel state))
-                   (t (er hard 'read-bytes$ "Bad case in read-bytes$.")))
-               (case bytes
-                 (1 `(read-byte$ ,channel state))
-                 (2 `(read-16ule ,channel state))
-                 (4 `(read-32ule ,channel state))
-                 (t (er hard 'read-bytes$ "Bad case in read-bytes$.")))))
-    (t (er hard 'read-bytes$ "Bad case in read-bytes$."))))
-
+                   (1 `(read-byte$ ,channel state))
+                   (2 `(read-16ule ,channel state))
+                   (4 `(read-32ule ,channel state))
+                   (8 `(read-64ule ,channel state))
+                   (t (er hard 'read-bytes$ "Bad case in read-bytes$.")))))
+      (t (er hard 'read-bytes$ "Bad case in read-bytes$.")))))
 
 
 
 
 ;; reading sequences of data
 
-(defmacro create-n-reader (read-1 fails?)
+(defmacro create-n-reader (read-1 fails? &key (short '""))
   (declare (xargs :guard (and (symbolp read-1)
-                              (booleanp fails?))))
+                              (booleanp fails?)
+                              (stringp short))))
   (let ((tr-read-n (intern-in-package-of-symbol
                     (concatenate 'string "TR-" (symbol-name read-1) "-N")
                     read-1))
@@ -823,50 +1003,52 @@
         (read-n-data (intern-in-package-of-symbol
                       (concatenate 'string (symbol-name read-1) "-N-DATA")
                       read-1)))
-    `(encapsulate
-      nil
-      (defun ,tr-read-n (n channel state acc)
-        (declare (xargs :guard (and (natp n)
-                                    (state-p state)
-                                    (symbolp channel)
-                                    (open-input-channel-p channel :byte state)
-                                    (true-listp acc))))
-        (if (mbe :logic (zp n) :exec (= 0 n))
-            (mv (reverse acc) state)
-          (mv-let (byte state)
-                  (,read-1 channel state)
-                  (cond ((eq byte nil)
-                         (mv 'fail state))
-                        ,@(if fails?
-                              `(((eq byte 'fail)
-                                (mv 'fail state)))
-                            nil)
-                        (t (,tr-read-n (1- n) channel state
-                                       (cons byte acc)))))))
+    `(defsection ,read-n
+       :parents (read-bytes$-n)
+       :short ,short
 
-      (defun ,read-n (n channel state)
-        (declare (xargs :guard (and (natp n)
-                                    (state-p state)
-                                    (symbolp channel)
-                                    (open-input-channel-p channel :byte state))
-                        :verify-guards nil))
-        (mbe :logic (if (zp n)
-                        (mv nil state)
-                      (mv-let (byte state)
-                              (,read-1 channel state)
-                              (cond ((eq byte nil)
-                                     (mv 'fail state))
-                                    ,@(if fails?
-                                          `(((eq byte 'fail)
-                                            (mv 'fail state)))
-                                        nil)
-                                    (t (mv-let (rest state)
-                                               (,read-n (1- n) channel state)
-                                               (mv (if (eq rest 'fail)
-                                                       'fail
-                                                     (cons byte rest))
-                                                   state))))))
-       :exec (,tr-read-n n channel state nil)))
+       (defun ,tr-read-n (n channel state acc)
+         (declare (xargs :guard (and (natp n)
+                                     (state-p state)
+                                     (symbolp channel)
+                                     (open-input-channel-p channel :byte state)
+                                     (true-listp acc))))
+         (if (mbe :logic (zp n) :exec (= 0 n))
+             (mv (reverse acc) state)
+           (mv-let (byte state)
+             (,read-1 channel state)
+             (cond ((eq byte nil)
+                    (mv 'fail state))
+                   ,@(if fails?
+                         `(((eq byte 'fail)
+                            (mv 'fail state)))
+                       nil)
+                   (t (,tr-read-n (1- n) channel state
+                                  (cons byte acc)))))))
+
+       (defun ,read-n (n channel state)
+         (declare (xargs :guard (and (natp n)
+                                     (state-p state)
+                                     (symbolp channel)
+                                     (open-input-channel-p channel :byte state))
+                         :verify-guards nil))
+         (mbe :logic (if (zp n)
+                         (mv nil state)
+                       (mv-let (byte state)
+                         (,read-1 channel state)
+                         (cond ((eq byte nil)
+                                (mv 'fail state))
+                               ,@(if fails?
+                                     `(((eq byte 'fail)
+                                        (mv 'fail state)))
+                                   nil)
+                               (t (mv-let (rest state)
+                                    (,read-n (1- n) channel state)
+                                    (mv (if (eq rest 'fail)
+                                            'fail
+                                          (cons byte rest))
+                                        state))))))
+              :exec (,tr-read-n n channel state nil)))
 
       (local (defthm lemma-decompose-impl
                (equal (,tr-read-n n channel state acc)
@@ -922,56 +1104,146 @@
         (implies (not (equal (mv-nth 0 (,read-n n channel state)) 'fail))
                  (and (true-listp (mv-nth 0 (,read-n n channel state)))
                       (equal (len (mv-nth 0 (,read-n n channel state)))
-                             (nfix n)))))
-
-)))
+                             (nfix n))))))))
 
 
+(create-n-reader read-byte$ nil
+                 :short "@(call read-byte$-n) reads @('n') unsigned bytes from
+                         the input channel and returns them as a list.")
 
-(create-n-reader read-byte$ nil)
-(create-n-reader read-8s nil)
-
-(create-n-reader read-16ube t)
-(create-n-reader read-16ule t)
-(create-n-reader read-16sbe t)
-(create-n-reader read-16sle t)
-
-(create-n-reader read-32ube t)
-(create-n-reader read-32ule t)
-(create-n-reader read-32sbe t)
-(create-n-reader read-32sle t)
+(create-n-reader read-8s nil
+                 :short "@(call read-8s-n) reads @('n') signed bytes from the
+                         input channel and returns them as a list.")
 
 
 
-(defmacro read-bytes$-n (n channel &key (bytes '1) (signed 'nil) (end 'big))
-  (declare (xargs :guard (and (symbolp channel)
-                              (booleanp signed)
-                              (or (equal bytes 1)
-                                  (equal bytes 2)
-                                  (equal bytes 4))
-                              (or (equal end 'little)
-                                  (equal end 'big)))))
-  (case end
-    ('big (if signed
+(create-n-reader read-16ube t
+                 :short "@(call read-16ube-n) reads @('n') 16-bit, unsigned,
+                         big-endian values from the input channel and returns
+                         them as a list.")
+
+(create-n-reader read-16ule t
+                 :short "@(call read-16ule-n) reads @('n') 16-bit, unsigned,
+                         little-endian values from the input channel and
+                         returns them as a list.")
+
+(create-n-reader read-16sbe t
+                 :short "@(call read-16sbe-n) reads @('n') 16-bit, signed,
+                         big-endian values from the input channel and returns
+                         them as a list.")
+
+(create-n-reader read-16sle t
+                 :short "@(call read-16sle-n) reads @('n') 16-bit, signed,
+                         little-endian values from the input channel and
+                         returns them as a list.")
+
+
+
+
+(create-n-reader read-32ube t
+                 :short "@(call read-32ube-n) reads @('n') 32-bit, unsigned,
+                         big-endian values from the input channel and returns
+                         them as a list.")
+
+(create-n-reader read-32ule t
+                 :short "@(call read-32ule-n) reads @('n') 32-bit, unsigned,
+                         little-endian values from the input channel and
+                         returns them as a list.")
+
+(create-n-reader read-32sbe t
+                 :short "@(call read-32sbe-n) reads @('n') 32-bit, signed,
+                         big-endian values from the input channel and returns
+                         them as a list.")
+
+(create-n-reader read-32sle t
+                 :short "@(call read-32sle-n) reads @('n') 32-bit, signed,
+                         little-endian values from the input channel and
+                         returns them as a list.")
+
+
+
+(create-n-reader read-64ube t
+                 :short "@(call read-64ube-n) reads @('n') 64-bit, unsigned,
+                         big-endian values from the input channel and returns
+                         them as a list.")
+
+(create-n-reader read-64ule t
+                 :short "@(call read-64ule-n) reads @('n') 64-bit, unsigned,
+                         little-endian values from the input channel and
+                         returns them as a list.")
+
+(create-n-reader read-64sbe t
+                 :short "@(call read-64sbe-n) reads @('n') 64-bit, signed,
+                         big-endian values from the input channel and returns
+                         them as a list.")
+
+(create-n-reader read-64sle t
+                 :short "@(call read-64sle-n) reads @('n') 64-bit, signed,
+                         little-endian values from the input channel and
+                         returns them as a list.")
+
+
+
+(defsection read-bytes$-n
+  :parents (io)
+  :short "Flexible macro for reading whole lists of @('n') 1-, 2-, 4-, or
+8-byte values from an open @(':byte') input stream."
+
+  :long "<p>General form:</p>
+
+@({
+     (read-bytes$-n n channel
+                    [:bytes bytes]     ;; default: 1
+                    [:signed signed]   ;; default: nil
+                    [:end end]         ;; default: big
+                    )
+})
+
+<p>The @('bytes'), @('signed'), and @('end') arguments are as in @(see
+read-bytes$).</p>
+
+<p>The number @('n') says how many values to read.  The actual number of bytes
+that will be read is therefore @('n * bytes').  E.g., reading three 8-byte
+values will consume a total of 24 bytes from the input stream.</p>
+
+<p>If EOF is reached before @('n * bytes') bytes are read from the stream, then
+we return @('fail').  Otherwise, we return an @('n')-element list, where every
+member is an appropriate integer for this combination of signedness and
+size.</p>"
+
+  (defmacro read-bytes$-n (n channel &key (bytes '1) (signed 'nil) (end 'big))
+    (declare (xargs :guard (and (symbolp channel)
+                                (booleanp signed)
+                                (or (equal bytes 1)
+                                    (equal bytes 2)
+                                    (equal bytes 4))
+                                (or (equal end 'little)
+                                    (equal end 'big)))))
+    (case end
+      ('big (if signed
+                (case bytes
+                  (1 `(read-8s-n ,n ,channel state))
+                  (2 `(read-16sbe-n ,n ,channel state))
+                  (4 `(read-32sbe-n ,n ,channel state))
+                  (8 `(read-64sbe-n ,n ,channel state))
+                  (t (er hard 'read-bytes$-n "Bad case in read-bytes$-n.")))
               (case bytes
-                (1 `(read-8s-n ,n ,channel state))
-                (2 `(read-16sbe-n ,n ,channel state))
-                (4 `(read-32sbe-n ,n ,channel state))
-                (t (er hard 'read-bytes$-n "Bad case in read-bytes$-n.")))
-            (case bytes
-              (1 `(read-byte$-n ,n ,channel state))
-              (2 `(read-16ube-n ,n ,channel state))
-              (4 `(read-32ube-n ,n ,channel state))
-              (t (er hard 'read-bytes$-n "Bad case in read-bytes$-n.")))))
-    ('little (if signed
+                (1 `(read-byte$-n ,n ,channel state))
+                (2 `(read-16ube-n ,n ,channel state))
+                (4 `(read-32ube-n ,n ,channel state))
+                (8 `(read-64ube-n ,n ,channel state))
+                (t (er hard 'read-bytes$-n "Bad case in read-bytes$-n.")))))
+      ('little (if signed
+                   (case bytes
+                     (1 `(read-8s-n ,n ,channel state))
+                     (2 `(read-16sle-n ,n ,channel state))
+                     (4 `(read-32sle-n ,n ,channel state))
+                     (8 `(read-64sle-n ,n ,channel state))
+                     (t (er hard 'read-bytes$-n "Bad case in read-bytes$-n.")))
                  (case bytes
-                   (1 `(read-8s-n ,n ,channel state))
-                   (2 `(read-16sle-n ,n ,channel state))
-                   (4 `(read-32sle-n ,n ,channel state))
-                   (t (er hard 'read-bytes$-n "Bad case in read-bytes$-n.")))
-               (case bytes
-                 (1 `(read-byte$-n ,n ,channel state))
-                 (2 `(read-16ule-n ,n ,channel state))
-                 (4 `(read-32ule-n ,n ,channel state))
-                 (t (er hard 'read-bytes$-n "Bad case in read-bytes$-n.")))))
-    (t (er hard 'read-bytes$-n "Bad case in read-bytes$-n."))))
+                   (1 `(read-byte$-n ,n ,channel state))
+                   (2 `(read-16ule-n ,n ,channel state))
+                   (4 `(read-32ule-n ,n ,channel state))
+                   (8 `(read-64ule-n ,n ,channel state))
+                   (t (er hard 'read-bytes$-n "Bad case in read-bytes$-n.")))))
+      (t (er hard 'read-bytes$-n "Bad case in read-bytes$-n.")))))
